---
title: "Influence function calculation for Brier score for event time data"
author: "Johan Sebastian Ohlendorff & Thomas Alexander Gerds"
date: '2022-06-07'
output: pdf_document
header-includes: \usepackage{graphicx, verbatim, fancyvrb, setspace, xspace, colortbl, longtable, amsmath, caption, xfrac, float, mathabx,bbm,algorithm2e}
---


\newcommand{\Xj}{\ensuremath{X^{\prime}}}
\newcommand{\xj}{\ensuremath{x^{\prime}}}
\newcommand{\AUC}{\ensuremath{\operatorname{AUC}}}
\newcommand{\Brier}{\ensuremath{\operatorname{Brier}}}
\newcommand{\survtau}{\ensuremath{\tilde S(\tau)}}
\newcommand{\hatsurvtau}{\ensuremath{\hat{\tilde{S}}(\tau)}}
\newcommand{\Htau}{\ensuremath{H(\tau)}}
\newcommand{\hatHtau}{\ensuremath{\hat H^{(i)}(\tau)}}

\newcommand{\Utau}{\ensuremath{U(\tau)}}
\newcommand{\hatUtau}{\ensuremath{\hat U^{(i)}(\tau)}}
\newcommand{\Vtau}{\ensuremath{V(\tau)}}
\newcommand{\hatVtau}{\ensuremath{\hat V^{(i)}(\tau)}}
\newcommand{\Wtau}{\ensuremath{W(\tau)}}
\newcommand{\hatWtau}{\ensuremath{\hat W^{(i)}(\tau)}}
\newcommand{\margprob}{\ensuremath{F}}
\newcommand{\hatmargprob}{\ensuremath{\hat{F}}}
\newcommand{\Zi}{\ensuremath{Z_i}}
\newcommand{\emp}{\ensuremath{I\negthickspace P_n}}
\newcommand{\ifauc}{\ensuremath{\mathrm{IF}_{\mathrm{AUC}}}}
\newcommand{\hatifauc}{\ensuremath{\mathrm{\widehat{IF}}_{\mathrm{AUC}}}}
\newcommand{\ifnu}{\ensuremath{\mathrm{IF}_{\nu}}}
\newcommand{\ifnuc}{\ensuremath{\mathrm{IF}^1_{\nu}}}
\newcommand{\hatifnu}{\ensuremath{\mathrm{\widehat{IF}}_{\nu}}}
\newcommand{\hatifnuc}{\ensuremath{\mathrm{\widehat{IF}}^1_{\nu}}}
\newcommand{\ifmu}{\ensuremath{\mathrm{IF}_{\mu}}}
\newcommand{\hatifmu}{\ensuremath{\mathrm{\widehat{IF}}_{\mu}}}
\newcommand{\ifmuc}{\ensuremath{\mathrm{IF}^1_{\mu}}}
\newcommand{\hatifmuc}{\ensuremath{\mathrm{\widehat{IF}}^1_{\mu}}}


```{r setup, include=FALSE}
knitr::opts_chunk$set(echo = TRUE)
```

## IF Calculation
To describe the situation with competing risks (and also survival) we introduce a
random variable \(D\in\{1,2\}\) which indicates the cause (i.e., type
of the event) observed at time \(T\) such that \(D=1\) means that the
event of interest occurred, and \(D=2\) that a competing risk
occurred. As in the survival setting we let \(Q\) denote the joint
probability measure of the uncensored data, \((T,D,X)\sim Q\), and $P$
the joint probability measure of the right censored data
$Z=(\tilde{T},\Delta,X) \sim P$ now with $\Delta=D 1_{\{T \leq C\}}$
taking values in the set \(\{0,1,2\}\). We are interested in the
following definition of the time-dependent discrimination measure for
cause 1. We can easily calculate the influence function for the Brier score, which can be written as: 
\begin{align*}
& \int\left\{1_{\{ t \leq \tau \}}-R(\tau \mid x)\right\}^{2} Q(d t, d x)\\
&=\int 1_{\{t \leqslant \tau\}}-21_{\{t \leqslant \tau\}} R(\tau \mid x)+R(\tau \mid x)^{2} Q(d t, d x) \\
&= \int 1_{\{t \leqslant \tau\}}(1-2 R(\tau \mid x)) Q(d t, d x)+\int R(\tau \mid x)^{2} Q(d x) \\
&=\int \frac{1_{\{t \leqslant \tau\}}}{G(t- |x)}(1-2 R(\tau \mid x)) P(d t, 1, d x) + \int R\left(\tau | x\right)^2 P(d x)
\end{align*}
We find
\begin{align*}
IC_{\Brier}(\tilde{T}_i,\Delta_i,X_i;\tau) &= \partial_{\varepsilon} \int \frac{1_{\{t \leqslant \tau\}}}{G(t- |x)}(1-2 R(\tau \mid x)) P_{\varepsilon}(d t, 1, d x) +\partial_{\varepsilon} \int R\left(\tau | x\right)^2 P_{\varepsilon}(d x) \\&=
\int 1_{\{t \leqslant \tau \}}(1-2 R(\tau \mid x)) \frac{d(\delta_{\left\{\tilde{T}_{i}, \Delta_i,X_i\right\}})(t, 1, x)+dP(t,1,x)\left[f_i(t-,x)-1\right]}{G(t- |x)} \\
&+ \int R\left(\tau | x\right)^2 (\delta_{\left\{\tilde{T}_{i}, \Delta_i,X_i\right\}}-P) \\
&=   1_{\{\tilde{T}_i \leqslant \tau, \Delta_i=1\}}(1-2 R(\tau \mid X_i)) \frac{1}{G(\tilde{T}_i- | X_i)}  \\
&+  \int 1_{\{t \leqslant \tau\}}(1-2 R(\tau \mid x)) f_i(t-,x) \frac{dP(t,1,x)}{G(t-|x)} + R\left(\tau | X_i \right)^2 \\
&- \int R\left(\tau | x\right)^2 dP(x)
- \int 1_{\{t \leqslant \tau\}}(1-2 R(\tau \mid x)) \frac{dP(t,1,x)}{G(t-|x)}
\end{align*}
The last term that is subtracted is the Brier score. Then using that 
$$
 f_i(t,x) = \frac{\mathbbm{1}_{\{\tilde{T_i} \leq t, \Delta_i = 0\}} \delta_{X_i}(x)}{G(\tilde{T_i}|X_i)S(\tilde{T_i}|X_i)} -\int_0^{\tilde{T}_i \wedge t} \frac{ \delta_{X_i}(x)dP(s,0 | x)}{G(s|X_i)^2S(s|X_i)^2}
$$
we see that (plugging in $f(t,x)$ instead of $f(t-,x)$!)
$$
\begin{aligned}
\int_X \int_0^\tau(1-2R(\tau|x))f_i(t-,x) \frac{P(dt,1,x)}{G(t-|x)} &= \int_X \int_0^\tau(1-2R(\tau|x))\left[\frac{\mathbbm{1}_{\{\tilde{T_i} \leq t, \Delta_i = 0\}} \delta_{X_i}(x)}{G(\tilde{T_i}|X_i)S(\tilde{T_i}|X_i)} -\int_0^{\tilde{T}_i \wedge t} \frac{ \delta_{X_i}(x)P(ds,0 | x)}{G(s|X_i)^2S(s|X_i)^2}\right] \frac{P(dt,1,x)}{G(t-|x)} \\
&= \int_0^\tau(1-2R(\tau|X_i))\left[\frac{\mathbbm{1}_{\{\tilde{T_i} \leq t, \Delta_i = 0\}} }{G(\tilde{T_i}|X_i)S(\tilde{T_i}|X_i)} -\int_0^{\tilde{T}_i \wedge t} \frac{ P(ds,0 | X_i)}{G(s|X_i)^2S(s|X_i)^2}\right] \frac{P(dt,1 | X_i)}{G(t-|X_i)} \\
&= (i) - (ii)
\end{aligned}
$$
where 
$$
\begin{aligned}
(i) &=\int_0^\tau(1-2R(\tau|X_i))\frac{\mathbbm{1}_{\{\tilde{T_i} \leq t, \Delta_i = 0\}} }{G(\tilde{T_i}|X_i)S(\tilde{T_i}|X_i)} \frac{P(dt,1 | X_i)}{G(t-|X_i)} \\
&= (1-2R(\tau|X_i))\frac{\mathbbm{1}_{\{\tilde{T}_i \leq \tau,\Delta_i = 0\}} }{G(\tilde{T_i}|X_i)S(\tilde{T_i}|X_i)} \int_{\tilde{T}_i}^\tau \frac{P(dt,1 | X_i)}{G(t-|X_i)} \\
&= (1-2R(\tau|X_i))\frac{\mathbbm{1}_{\{\tilde{T}_i \leq \tau,\Delta_i = 0\}} }{G(\tilde{T_i}|X_i)S(\tilde{T_i}|X_i)} (F_1(\tau|X_i)-F_1(\tilde{T}_i|X_i))
\end{aligned}
$$

Similarly, we have
$$
\begin{aligned}
(ii) &=(1-2R(\tau|X_i))\int_0^\tau\int_0^{\tilde{T}_i \wedge t} \frac{ P(ds,0 | X_i)}{G(s|X_i)^2S(s|X_i)^2} \frac{P(dt,1 | X_i)}{G(t-|X_i)} \\
\end{aligned}
$$
If $\tilde{T}_i > \tau$, then this can be written as 
$$
\begin{aligned}
(ii) &=(1-2R(\tau|X_i))\int_0^\tau\int_s^{\tau} \frac{ P(dt,1 | X_i)}{G(t-|X_i)} \frac{P(ds,0 | X_i)}{G(s|X_i)^2S(s|X_i)^2} \\
&= (1-2R(\tau|X_i))\int_0^\tau(F_1(\tau|X_i)-F_1(s|X_i)) \frac{P(ds,0 | X_i)}{G(s|X_i)^2S(s|X_i)^2} 
\end{aligned}
$$
On the other hand, if $\tilde{T}_i \leq \tau$, then
$$
\begin{aligned}
(ii) &=(1-2R(\tau|X_i))\int_0^{\tilde{T}_i}\int_s^{\tau} \frac{ P(dt,1 | X_i)}{G(t-|X_i)} \frac{P(ds,0 | X_i)}{G(s|X_i)^2S(s|X_i)^2}  \\
&= (1-2R(\tau|X_i))\int_0^{\tilde{T}_i}(F_1(\tau|X_i)-F_1(s|X_i)) \frac{P(ds,0 | X_i)}{G(s|X_i)^2S(s|X_i)^2} 
\end{aligned}
$$
Thus 
$$
\begin{aligned}
(ii) 
&= (1-2R(\tau|X_i))\int_0^{\tilde{T}_i \wedge \tau}(F_1(\tau|X_i)-F_1(s|X_i)) \frac{P(ds,0 | X_i)}{G(s|X_i)^2S(s|X_i)^2} 
\end{aligned}
$$
Hence, 
$$
(i)-(ii) = (1-2R(\tau |X_i))\left(\frac{I(\tilde{T}_i \leq \tau, \Delta_i = 0)}{G(\tilde{T}_i|X_i)S(\tilde{T}_i|X_i)}(F_1(\tau|X_i)-F_1(\tilde{T}_i|X_i))-\int_0^{\tilde{T}_i \wedge \tau} \frac{(F_1(\tau|X_i)-F_1(s|X_i))}{G(s|X_i)^2S(s|X_i)^2}P(ds,0|X_i)\right)
$$


